src/FrameStack/Vulnerabilities/AtomExhaustion2.v
@@ -1,4 +1,4 @@
-From CoreErlang.FrameStack Require Import SubstSemantics.
+From CoreErlang.FrameStack Require Import SubstSemanticsLabeled.
 From stdpp Require Export gmap sets.
 
 Open Scope string_scope.
@@ -7,61 +7,24 @@ Module AtomExhaustion.
 
 Import ListNotations.
 
-Definition step_any_non_final (fs : FrameStack) (e : Redex) (fs' : FrameStack) (e' : Redex) : Prop :=
-  exists k, ⟨fs, e⟩ -[k]-> ⟨fs', e'⟩.
-Notation "⟨ fs , e ⟩ -->* ⟨ fs' , e' ⟩" := (step_any_non_final fs e fs' e').
-
-Inductive atom_generating_cfg : FrameStack -> Redex -> Prop :=
-| list_to_atom_frame fs (vl : list Val) (v : Val) (vs' : ValSeq) (eff' : SideEffectList):
-  Some ((RValSeq vs'), eff') =
-    create_result (ICall (VLit "erlang") (VLit "list_to_atom")) (vl ++ [v]) [] ->
-  (atom_generating_cfg
-    (FParams (ICall (VLit "erlang") (VLit "list_to_atom")) vl [] :: fs)
-    (RValSeq [v])).
-
-Definition atom_generating_step (fs: FrameStack) (r: Redex) (fs': FrameStack) (r': Redex) : Prop :=
-  (atom_generating_cfg fs r) /\ ⟨ fs , r ⟩ --> ⟨ fs' , r' ⟩.
-
-Definition generated_atom_value
-  (fs: FrameStack) (r: Redex) : option (string) :=
-match fs, r with
-| (FParams (ICall (VLit "erlang") (VLit "list_to_atom")) vl [] :: fs), (RValSeq [v])
-  =>
-  match create_result (ICall (VLit "erlang") (VLit "list_to_atom")) (vl ++ [v]) [] with
-  | Some ((RValSeq [VLit (Atom atom_val)]), eff') => Some atom_val
-  | _ => None
-  end
-| _, _ => None
-end.
-
-Goal generated_atom_value
-  [FParams (ICall (VLit "erlang") (VLit "list_to_atom")) [] []]
-  (RValSeq
-    [VCons (VLit 104%Z) (VCons (VLit 101%Z) (VCons (VLit 108%Z)
-    (VCons (VLit 108%Z) (VCons (VLit 111%Z) VNil))))]) = Some "hello".
-Proof.
-  simpl. reflexivity.
-Qed.
-
 Inductive generates_at_least_n_unique_atoms :
   FrameStack -> Redex -> gset string -> nat -> Prop :=
 | generates_terminal fs r s:
   generates_at_least_n_unique_atoms fs r s 0
 
-| generates_step_false fs r s n fs' r':
-  ⟨ fs , r ⟩ --> ⟨ fs' , r' ⟩ ->
+| generates_step_false fs r l fs' r' s n:
+  ⟨ fs , r ⟩ -⌊ l ⌋-> ⟨ fs' , r' ⟩ ->
   (generates_at_least_n_unique_atoms fs' r' s n) ->
   generates_at_least_n_unique_atoms fs r s n
 
-| generates_step_true_not_unique fs r s n fs' r' (av: string):
-  (Some av) = generated_atom_value fs r -> (* gset_elem_of av s -> *)
-  ⟨ fs , r ⟩ --> ⟨ fs' , r' ⟩ ->
+| generates_step_true_not_unique fs r (av: string) fs' r' s n:
+  ⟨ fs , r ⟩ -⌊ Some (AtomCreation, [VLit (Atom av)]) ⌋-> ⟨ fs' , r' ⟩ ->
   (generates_at_least_n_unique_atoms fs' r' s n) ->
   generates_at_least_n_unique_atoms fs r s n
 
-| generates_step_true_unique fs r s n fs' r' (av: string):
-  (Some av) = generated_atom_value fs r -> ¬(elem_of av s) ->
-  ⟨ fs , r ⟩ --> ⟨ fs' , r' ⟩ ->
+| generates_step_true_unique fs r (av: string) fs' r' s n:
+  ⟨ fs , r ⟩ -⌊ Some (AtomCreation, [VLit (Atom av)]) ⌋-> ⟨ fs' , r' ⟩ ->
+  av ∉ s ->
   (generates_at_least_n_unique_atoms fs' r' ({[av]} ∪ s) n) ->
   generates_at_least_n_unique_atoms fs r s (S n).
 
@@ -74,13 +37,11 @@ Ltac do_step := econstructor; [constructor; auto|simpl].
 Ltac apply_proper_constr := 
   eapply generates_terminal || (
   eapply generates_step_true_unique;
-    [simpl; reflexivity
-    | set_solver
-    | econstructor; reflexivity
+    [econstructor; reflexivity
+    |set_solver 
     |] || (
   eapply generates_step_true_not_unique;
-    [simpl; reflexivity
-    | econstructor; reflexivity
+    [econstructor; reflexivity
     |] ||
   eapply generates_step_false;
     [econstructor; try (scope_solver || congruence)
